finished section 3.4

analysis/Analysis/Section_3_4.lean
@@ -39,10 +39,47 @@ theorem SetTheory.Set.mem_image {X Y:Set} (f:X → Y) (S: Set) (y:Object) :
     y ∈ image f S ↔ ∃ x:X, x.val ∈ S ∧ f x = y := by
   grind [replacement_axiom]
 
+@[simp]
+theorem SetTheory.Set.image_singleton {X Y:Set} {f:X → Y} {x: Object} (h: x ∈ X) :
+  image f {x} = {↑(f ⟨x, h⟩)} := by
+    ext y
+    rw [mem_singleton, mem_image]
+    refine ⟨?_, fun hy => ⟨⟨x, h⟩, mem_singleton _ _ |>.mpr rfl, hy.symm⟩⟩ 
+    rintro ⟨x', hx, hfx⟩ 
+    exact (mem_singleton _ _ |>.mp hx) ▸  hfx.symm
+
+@[simp]
+theorem SetTheory.Set.image_singleton' {X Y:Set} (f:X → Y) (x: X) :
+  image f {x.val} = {↑(f x)} := image_singleton x.property
+
+@[simp]
+theorem SetTheory.Set.image_pair {X Y:Set} {f:X → Y} {x1 x2: Object} (h1: x1 ∈ X) (h2: x2 ∈ X):
+  image f {x1, x2} = {↑(f ⟨x1, h1⟩), ↑(f ⟨x2, h2⟩) } := by
+    ext y
+    rw [mem_pair, mem_image]
+    constructor
+    · rintro ⟨x, hx, hfx⟩ 
+      obtain (hx|hx) := mem_pair _ _ _ |>.mp hx
+      exact Or.inl <| hx ▸ hfx.symm
+      exact Or.inr <| hx ▸ hfx.symm
+    · rintro (hx|hx) 
+      exact ⟨⟨x1, h1⟩, mem_pair _ _ _ |>.mpr (Or.inl rfl), hx.symm⟩ 
+      exact ⟨⟨x2, h2⟩, mem_pair _ _ _ |>.mpr (Or.inr rfl), hx.symm⟩ 
+
+@[simp]
+theorem SetTheory.Set.image_pair' {X Y:Set} (f:X → Y) (x1 x2: X) :
+  image f {x1.val, x2.val} = {↑(f x1), ↑(f x2)} := image_pair x1.property x2.property
+
 /-- Alternate definition of image using axiom of specification -/
 theorem SetTheory.Set.image_eq_specify {X Y:Set} (f:X → Y) (S: Set) :
-    image f S = Y.specify (fun y ↦ ∃ x:X, x.val ∈ S ∧ f x = y) := by sorry
-
+  image f S = Y.specify (fun y ↦ ∃ x:X, x.val ∈ S ∧ f x = y) := by
+    refine Set.ext_iff.mpr fun y => ?_
+    rw [mem_image, specification_axiom'']
+    constructor
+    · refine fun ⟨x, hx, hfx⟩ => ⟨?_, x, hx, ?_⟩ 
+      exact hfx ▸ subtype_property _ _
+      exact (coe_inj _ _ _).mp hfx
+    · exact fun ⟨hy, x, hx, hfx⟩ => ⟨x, hx, hfx ▸ rfl⟩ 
 /--
   Connection with Mathlib's notion of image.  Note the need to utilize the `Subtype.val` coercion
   to make everything type consistent.
@@ -52,7 +89,7 @@ theorem SetTheory.Set.image_eq_image {X Y:Set} (f:X → Y) (S: Set):
   ext; simp; grind
 
 theorem SetTheory.Set.image_in_codomain {X Y:Set} (f:X → Y) (S: Set) :
-    image f S ⊆ Y := by intro _ h; rw [mem_image] at h; grind
+    image f S ⊆ Y := by intro _ h; rw [mem_image] at h; grind only [cases eager Subtype]
 
 /-- Example 3.4.2 -/
 abbrev f_3_4_2 : nat → nat := fun n ↦ (2*n:ℕ)
@@ -68,16 +105,22 @@ theorem SetTheory.Set.image_f_3_4_2 : image f_3_4_2 {1,2,3} = {2,4,6} := by
 example : (fun n:ℤ ↦ n^2) '' {-1,0,1,2} = {0,1,4} := by aesop
 
 theorem SetTheory.Set.mem_image_of_eval {X Y:Set} (f:X → Y) (S: Set) (x:X) :
-    x.val ∈ S → (f x).val ∈ image f S := by sorry
+  x.val ∈ S → (f x).val ∈ image f S :=
+    fun hx => mem_image _ _ _ |>.mpr ⟨x, hx, rfl⟩ 
+
 
 theorem SetTheory.Set.mem_image_of_eval_counter :
-    ∃ (X Y:Set) (f:X → Y) (S: Set) (x:X), ¬((f x).val ∈ image f S → x.val ∈ S) := by sorry
+  ∃ (X Y:Set) (f:X → Y) (S: Set) (x:X), ¬((f x).val ∈ image f S → x.val ∈ S) := by
+    use {0, 1}, {0}, Function.const _ ⟨0, mem_singleton _ _ |>.mpr rfl⟩
+    use {1}, ⟨0, mem_pair _ _ _ |>.mpr (Or.inl rfl)⟩ 
+    simp
 
 /--
   Definition 3.4.4 (inverse images).
   Again, it is not required that U be a subset of Y.
 -/
-abbrev SetTheory.Set.preimage {X Y:Set} (f:X → Y) (U: Set) : Set := X.specify (P := fun x ↦ (f x).val ∈ U)
+abbrev SetTheory.Set.preimage {X Y:Set} (f:X → Y) (U: Set) : Set := 
+  X.specify (P := fun x ↦ (f x).val ∈ U)
 
 @[simp]
 theorem SetTheory.Set.mem_preimage {X Y:Set} (f:X → Y) (U: Set) (x:X) :
@@ -110,7 +153,25 @@ theorem SetTheory.Set.preimage_f_3_4_2 : preimage f_3_4_2 {2,4,6} = {1,2,3} := b
   all_goals simp
 
 theorem SetTheory.Set.image_preimage_f_3_4_2 :
-    image f_3_4_2 (preimage f_3_4_2 {1,2,3}) ≠ {1,2,3} := by sorry
+  image f_3_4_2 (preimage f_3_4_2 {1,2,3}) ≠ {1,2,3} := by
+    rw [show preimage f_3_4_2 {1,2,3} = {1} by
+      ext x
+      simp only [mem_preimage', mem_triple, mem_singleton, f_3_4_2]
+      constructor
+      · rintro ⟨x, rfl, (_ | _ | _)⟩ <;> simp_all; omega
+      rintro (rfl | rfl | rfl)
+      all_goals simp
+      refine ⟨(1: Nat), (1: Nat).prop, by simp⟩,
+    show image f_3_4_2 {1} = {2} by
+      ext x
+      simp
+    ]
+    by_contra! h
+    rw [Set.ext_iff] at h
+    have := h (1: ℕ) |>.mpr (mem_triple _ _ _ _ |>.mpr (Or.inl rfl)) |> (mem_singleton _ _).mp
+    rw [show (2: Object) = ↑(2 : ℕ) by rfl] at this
+    replace : (1 : ℕ) = (2: ℕ) := (ofNat_inj' 1 2).mp this
+    contradiction
 
 /-- Example 3.4.7 (using the Mathlib notion of preimage) -/
 example : (fun n:ℤ ↦ n^2) ⁻¹' {0,1,4} = {-2,-1,0,1,2} := by
@@ -118,7 +179,20 @@ example : (fun n:ℤ ↦ n^2) ⁻¹' {0,1,4} = {-2,-1,0,1,2} := by
   on_goal 3 => have : 2 ^ 2 = (4:ℤ) := (by norm_num); rw [←h, sq_eq_sq_iff_eq_or_eq_neg] at this
   all_goals aesop
 
-example : (fun n:ℤ ↦ n^2) ⁻¹' ((fun n:ℤ ↦ n^2) '' {-1,0,1,2}) ≠ {-1,0,1,2} := by sorry
+example : (fun n:ℤ ↦ n^2) ⁻¹' ((fun n:ℤ ↦ n^2) '' {-1,0,1,2}) ≠ {-1,0,1,2} := by
+  rw [show (fun n:ℤ ↦ n^2) '' {-1,0,1,2} = {0, 1, 4} by aesop,
+    show (fun n ↦ n ^ 2) ⁻¹' {0, 1, 4} = {-2, -1, 0, 1, 2} by
+      ext x
+      rw [_root_.Set.mem_preimage]
+      simp only [Set.mem_insert_iff, ne_eq, OfNat.ofNat_ne_zero, not_false_eq_true, pow_eq_zero_iff,
+        sq_eq_one_iff, Int.reduceNeg, Set.mem_singleton_iff]
+      rw [show (4: ℤ) = 2 ^ 2 by norm_num, sq_eq_sq_iff_eq_or_eq_neg]
+      tauto
+  ]
+  by_contra h
+  have : (-2 : ℤ) ∉ ({-1, 0, 1, 2}: _root_.Set ℤ) := of_decide_eq_false rfl
+  exact (h ▸ this) (Set.mem_insert _ _)
+
 
 instance SetTheory.Set.inst_pow : Pow Set Set where
   pow := pow
@@ -162,20 +236,37 @@ theorem SetTheory.Set.example_3_4_9 (F:Object) :
   rintro ⟨f, rfl⟩
   have h1 := (f ⟨4, by simp⟩).property
   have h2 := (f ⟨7, by simp⟩).property
-  simp [coe_of_fun_inj] at *
+  simp only [mem_insert, mem_singleton, coe_of_fun_inj] at *
   obtain _ | _ := h1 <;> obtain _ | _ := h2
   map_tacs [left; (right;left); (right;right;left); (right;right;right)]
   all_goals ext ⟨_, hx⟩; simp at hx; grind
 
 /-- Exercise 3.4.6 (i). One needs to provide a suitable definition of the power set here. -/
 def SetTheory.Set.powerset (X:Set) : Set :=
-  (({0,1} ^ X): Set).replace (P := sorry) (by sorry)
+  (({0,1} ^ X): Set).replace (P := fun F Y =>
+    ∃(f : X.toSubtype → ({0,1} : Set).toSubtype), F = (f: Object) ∧ Y = preimage f {1}
+  ) (by aesop)
 
 open Classical in
 /-- Exercise 3.4.6 (i) -/
 @[simp]
 theorem SetTheory.Set.mem_powerset {X:Set} (x:Object) :
-    x ∈ powerset X ↔ ∃ Y:Set, x = Y ∧ Y ⊆ X := by sorry
+  x ∈ powerset X ↔ ∃ Y:Set, x = Y ∧ Y ⊆ X := by
+    simp [powerset, replacement_axiom]
+    constructor
+    · rintro ⟨Y, rfl⟩ 
+      exact ⟨preimage Y {1}, rfl, preimage_in_domain _ _⟩
+    rintro ⟨Y, rfl, hY⟩ 
+    use fun x => if x.val ∈ Y 
+      then ⟨1, mem_pair _ _ _ |>.mpr (Or.inr rfl)⟩ 
+      else ⟨0, mem_pair _ _ _ |>.mpr (Or.inl rfl)⟩
+    refine (coe_eq_iff _ _).mpr ?_
+    ext y
+    refine ⟨fun hy => ?_, ?_⟩ 
+    · have : y = ↑(⟨y, hY _ hy⟩: X.toSubtype) := rfl
+      rw [this, mem_preimage]
+      simp [hy]
+    · aesop
 
 /-- Lemma 3.4.10 -/
 theorem SetTheory.Set.exists_powerset (X:Set) :
@@ -212,10 +303,29 @@ theorem SetTheory.Set.powerset_of_triple (a b c x:Object) :
 theorem SetTheory.Set.union_axiom (A: Set) (x:Object) :
     x ∈ union A ↔ ∃ (S:Set), x ∈ S ∧ (S:Object) ∈ A := SetTheory.union_axiom A x
 
+theorem SetTheory.Set.union_empty_eq : union ∅ = ∅ := by
+  ext x
+  rw [union_axiom, iff_false_right (not_mem_empty _), not_exists]
+  intro S
+  rw [not_and]
+  exact fun _ hS => (not_mem_empty _) hS
+
 /-- Example 3.4.12 -/
 theorem SetTheory.Set.example_3_4_12 :
     union { (({2,3}:Set):Object), (({3,4}:Set):Object), (({4,5}:Set):Object) } = {2,3,4,5} := by
-  sorry
+  ext x
+  rw [union_axiom, show x ∈ ({2, 3, 4, 5}: Set) ↔ x = 2 ∨ x = 3 ∨ x = 4 ∨ x = 5 by
+    simp_rw [Set.mem_insert, Set.mem_singleton]]
+  constructor
+  · rintro ⟨S, hx, hS⟩ 
+    obtain (hS|hS|hS):= mem_triple _ _ _ _ |>.mp hS
+    <;> obtain hS|hS := mem_pair _ _ _ |>.mp ((set_to_object.inj' hS ) ▸ hx)
+    <;> simp [hS]
+  · rintro (rfl|rfl|rfl|rfl)
+    · use {2,3}; simp
+    · use {2,3}; simp
+    · use {4,5}; simp
+    · use {4,5}; simp
 
 /-- Connection with Mathlib union -/
 theorem SetTheory.Set.union_eq (A: Set) :
@@ -247,7 +357,9 @@ theorem SetTheory.Set.iUnion_eq (I: Set) (A: I → Set) :
     (iUnion I A : _root_.Set Object) = ⋃ α, (A α: _root_.Set Object) := by
   ext; simp [mem_iUnion]
 
-theorem SetTheory.Set.iUnion_of_empty (A: (∅:Set) → Set) : iUnion (∅:Set) A = ∅ := by sorry
+theorem SetTheory.Set.iUnion_of_empty (A: (∅:Set) → Set) : iUnion (∅:Set) A = ∅ := by
+  ext x
+  rw [iUnion, replace_empty, union_empty_eq]
 
 /-- Indexed intersection -/
 noncomputable abbrev SetTheory.Set.nonempty_choose {I:Set} (hI: I ≠ ∅) : I :=
@@ -261,61 +373,265 @@ noncomputable abbrev SetTheory.Set.iInter (I: Set) (hI: I ≠ ∅) (A: I → Set
 
 theorem SetTheory.Set.mem_iInter {I:Set} (hI: I ≠ ∅) (A: I → Set) (x:Object) :
     x ∈ iInter I hI A ↔ ∀ α:I, x ∈ A α := by
-  sorry
+  rw [specification_axiom'']
+  constructor
+  · rintro ⟨hx, h⟩ a
+    exact h a
+  · intro h
+    refine ⟨h (nonempty_choose hI), fun α ↦ h α⟩
 
 /-- Exercise 3.4.1 -/
 theorem SetTheory.Set.preimage_eq_image_of_inv {X Y V:Set} (f:X → Y) (f_inv: Y → X)
-  (hf: Function.LeftInverse f_inv f ∧ Function.RightInverse f_inv f) (hV: V ⊆ Y) :
-    image f_inv V = preimage f V := by sorry
+  (hf: Function.LeftInverse f_inv f ∧ Function.RightInverse f_inv f) (_hV: V ⊆ Y) :
+  image f_inv V = preimage f V := by
+    ext x
+    rw [mem_image, mem_preimage']
+    refine ⟨fun ⟨y',hV, hfy⟩ => ?_, ?_⟩ 
+    · use f_inv y', hfy, hf.right y' |>.symm ▸ hV
+    rintro ⟨x, rfl, hV⟩ 
+    use f x, hV, hf.left x |>.symm ▸ rfl
 
 /- Exercise 3.4.2.  State and prove an assertion connecting `preimage f (image f S)` and `S`. -/
--- theorem SetTheory.Set.preimage_of_image {X Y:Set} (f:X → Y) (S: Set) (hS: S ⊆ X) : sorry := by sorry
+theorem SetTheory.Set.preimage_of_image {X Y:Set} (f:X → Y) (S: Set) (hS: S ⊆ X) 
+  : S ⊆ preimage f (image f S) := by
+    intro x hx
+    rw [mem_preimage']
+    use ⟨x, hS _ hx⟩, rfl
+    rw [mem_image]
+    use ⟨x, hS _ hx⟩
+
 
 /- Exercise 3.4.2.  State and prove an assertion connecting `image f (preimage f U)` and `U`.
 Interestingly, it is not needed for U to be a subset of Y. -/
--- theorem SetTheory.Set.image_of_preimage {X Y:Set} (f:X → Y) (U: Set) : sorry := by sorry
+theorem SetTheory.Set.image_of_preimage {X Y:Set} (f:X → Y) (U: Set) :
+  image f (preimage f U) ⊆ U := by
+    intro x
+    rw [mem_image]
+    intro ⟨y, h, hy⟩ 
+    exact hy ▸ (mem_preimage _ _ _ |>.mp h)
 
 /- Exercise 3.4.2.  State and prove an assertion connecting `preimage f (image f (preimage f U))` and `preimage f U`.
 Interestingly, it is not needed for U to be a subset of Y.-/
--- theorem SetTheory.Set.preimage_of_image_of_preimage {X Y:Set} (f:X → Y) (U: Set) : sorry := by sorry
+theorem SetTheory.Set.preimage_of_image_of_preimage {X Y:Set} (f:X → Y) (U: Set) : 
+  preimage f (image f (preimage f U)) = preimage f U := by
+    ext x
+    rw [mem_preimage', mem_preimage']
+    constructor
+    · rintro ⟨x, rfl, hx⟩ 
+      use x, rfl, image_of_preimage _ _ _ hx
+    · rintro ⟨x, rfl, hx⟩ 
+      refine ⟨x, rfl, ?_⟩
+      rw [mem_image]
+      refine ⟨x, ?_, rfl⟩
+      rw [mem_preimage]
+      exact hx
 
 /--
   Exercise 3.4.3.
 -/
 theorem SetTheory.Set.image_of_inter {X Y:Set} (f:X → Y) (A B: Set) :
-    image f (A ∩ B) ⊆ (image f A) ∩ (image f B) := by sorry
+  image f (A ∩ B) ⊆ (image f A) ∩ (image f B) := by
+    intro x hx
+    rw [mem_inter]
+    simp_rw [mem_image] at hx ⊢
+    obtain ⟨x, hx, hfx⟩ := hx
+    refine ⟨⟨x, ?_, hfx⟩, ⟨x, ?_, hfx⟩⟩ 
+    · exact mem_inter _ _ _ |>.mp hx |>.left
+    · exact mem_inter _ _ _ |>.mp hx |>.right
 
 theorem SetTheory.Set.image_of_diff {X Y:Set} (f:X → Y) (A B: Set) :
-    (image f A) \ (image f B) ⊆ image f (A \ B) := by sorry
+  (image f A) \ (image f B) ⊆ image f (A \ B) := by
+    intro x hx
+    rw [mem_sdiff] at hx
+    simp_rw [mem_image] at hx ⊢
+    push_neg at hx
+    obtain ⟨⟨x, hx, hfx⟩, hb⟩ := hx
+    have : x.val ∉ B := fun hB => hb x hB hfx
+    refine ⟨x, mem_sdiff _ _ _ |>.mpr ⟨hx, this⟩, hfx⟩ 
 
 theorem SetTheory.Set.image_of_union {X Y:Set} (f:X → Y) (A B: Set) :
-    image f (A ∪ B) = (image f A) ∪ (image f B) := by sorry
+  image f (A ∪ B) = (image f A) ∪ (image f B) := by
+    ext x
+    simp_rw [mem_union, mem_image]
+    constructor
+    · rintro ⟨x, hx, hfx⟩ 
+      rcases mem_union _ _ _ |>.mp hx with hx|hx
+      exact Or.inl ⟨x, hx, hfx⟩ 
+      exact Or.inr ⟨x, hx, hfx⟩ 
+    · rintro (⟨x, hx, hfx⟩|⟨x, hx, hfx⟩) 
+      exact ⟨x, mem_union _ _ _ |>.mpr (Or.inl hx), hfx⟩ 
+      exact ⟨x, mem_union _ _ _ |>.mpr (Or.inr hx), hfx⟩ 
 
+open Classical in
 def SetTheory.Set.image_of_inter' : Decidable (∀ X Y:Set, ∀ f:X → Y, ∀ A B: Set, image f (A ∩ B) = (image f A) ∩ (image f B)) := by
   -- The first line of this construction should be either `apply isTrue` or `apply isFalse`
-  sorry
+  apply isFalse
+  push_neg
+  have h0o: (0: Object) ∈ ({0, 1}: Set) := mem_pair _ _ _ |>.mpr (Or.inl rfl)
+  have h1o: (1: Object) ∈ ({0, 1}: Set) := mem_pair _ _ _ |>.mpr (Or.inr rfl)
+  have h0: (0: Object) ∈ ({0, 1, 2}: Set) := mem_triple _ _ _ _ |>.mpr (Or.inl rfl)
+  have h1: (1: Object) ∈ ({0, 1, 2}: Set) := mem_triple _ _ _ _ |>.mpr (Or.inr <| Or.inl rfl)
+  have h2: (2: Object) ∈ ({0, 1, 2}: Set) := mem_triple _ _ _ _ |>.mpr (Or.inr <| Or.inr rfl)
+  let f : ({0, 1, 2}: Set).toSubtype → ({0, 1}: Set).toSubtype := 
+    fun x => if x = ⟨1, h1⟩  then ⟨1, h1o⟩  else ⟨0, h0o⟩
+  have hf0 : ↑(f ⟨0, h0⟩) = (0: Object) := by
+    unfold f
+    rw [if_neg]
+    simp
+  have hf1 : ↑(f ⟨1, h1⟩) = (1: Object) := by
+    unfold f
+    rw [if_pos]
+    simp
+  have hf2 : ↑(f ⟨2, h2⟩) = (0: Object) := by 
+    unfold f
+    rw [if_neg]
+    simp
+  use {0, 1, 2}, {0, 1}, f
+  use {0, 1}, {1, 2}
+  rw [
+    show ({0,1}: Set) ∩ {1,2} = {1} by
+      ext x
+      rw [pair_comm, mem_inter, mem_pair, mem_pair, mem_singleton, ← or_and_left, or_iff_left]
+      aesop,
+    image_singleton h1,
+    image_pair h0 h1,
+    image_pair h1 h2,
+    hf0,
+    hf1,
+    hf2,
+    pair_comm,
+    inter_self,
+    not_eq_iff
+  ]
+  use 0
+  apply iff_not_comm.mp
+  exact ⟨
+    fun _ hx => (show (0: Object) ≠ 1 by norm_num) <| mem_singleton _ _ |>.mp hx,
+    fun _ => mem_pair _ _ _ |>.mpr (Or.inr rfl)⟩ 
 
+open Classical in
 def SetTheory.Set.image_of_diff' : Decidable (∀ X Y:Set, ∀ f:X → Y, ∀ A B: Set, image f (A \ B) = (image f A) \ (image f B)) := by
   -- The first line of this construction should be either `apply isTrue` or `apply isFalse`
-  sorry
+  apply isFalse
+  push_neg
+  have h0o: (0: Object) ∈ ({0, 1}: Set) := mem_pair _ _ _ |>.mpr (Or.inl rfl)
+  have h1o: (1: Object) ∈ ({0, 1}: Set) := mem_pair _ _ _ |>.mpr (Or.inr rfl)
+  have h0: (0: Object) ∈ ({0, 1, 2}: Set) := mem_triple _ _ _ _ |>.mpr (Or.inl rfl)
+  have h1: (1: Object) ∈ ({0, 1, 2}: Set) := mem_triple _ _ _ _ |>.mpr (Or.inr <| Or.inl rfl)
+  have h2: (2: Object) ∈ ({0, 1, 2}: Set) := mem_triple _ _ _ _ |>.mpr (Or.inr <| Or.inr rfl)
+  let f : ({0, 1, 2}: Set).toSubtype → ({0, 1}: Set).toSubtype := 
+    fun x => if x = ⟨1, h1⟩  then ⟨1, h1o⟩  else ⟨0, h0o⟩
+  have hf0 : ↑(f ⟨0, h0⟩) = (0: Object) := by
+    unfold f
+    rw [if_neg]
+    simp
+  have hf1 : ↑(f ⟨1, h1⟩) = (1: Object) := by
+    unfold f
+    rw [if_pos]
+    simp
+  have hf2 : ↑(f ⟨2, h2⟩) = (0: Object) := by 
+    unfold f
+    rw [if_neg]
+    simp
+  use {0, 1, 2}, {0, 1}, f
+  use {0, 1}, {1, 2}
+  rw [show ({0, 1}: Set) \ {1, 2} = {0} by aesop]
+  simp only [mem_insert, ofNat_inj', zero_ne_one, mem_singleton, OfNat.zero_ne_ofNat, or_self,
+    or_false, image_singleton, hf0, one_ne_zero, OfNat.one_ne_ofNat, or_true, image_pair, hf1,
+    OfNat.ofNat_ne_zero, OfNat.ofNat_ne_one, hf2]
+  rw [show ({0, 1}: Set) \ {1, 0} = {} by aesop, not_eq_iff]
+  refine ⟨0, fun _ => not_mem_empty _, fun _ => ?_⟩
+  exact mem_singleton _ _ |>.mpr rfl
 
 /-- Exercise 3.4.4 -/
 theorem SetTheory.Set.preimage_of_inter {X Y:Set} (f:X → Y) (A B: Set) :
-    preimage f (A ∩ B) = (preimage f A) ∩ (preimage f B) := by sorry
+  preimage f (A ∩ B) = (preimage f A) ∩ (preimage f B) := by
+    ext x
+    simp_rw [mem_inter, mem_preimage']
+    constructor
+    · rintro ⟨x, hx, h⟩ 
+      rw [mem_inter] at h
+      refine ⟨⟨x, hx, h.left⟩, ⟨x, hx, h.right⟩⟩ 
+    · rintro ⟨⟨x, hx, h_l⟩,⟨x', hx', h_r⟩⟩ 
+      obtain rfl : x = x' := coe_inj _ _ _ |>.mp (hx ▸ hx'.symm)
+      use x, hx, mem_inter _ _ _ |>.mpr ⟨h_l, h_r⟩ 
+
 
 theorem SetTheory.Set.preimage_of_union {X Y:Set} (f:X → Y) (A B: Set) :
-    preimage f (A ∪ B) = (preimage f A) ∪ (preimage f B) := by sorry
+  preimage f (A ∪ B) = (preimage f A) ∪ (preimage f B) := by
+    ext x
+    simp_rw [mem_union, mem_preimage']
+    constructor
+    · rintro ⟨x, hx, hfx⟩ 
+      rcases mem_union _ _ _ |>.mp hfx with hfx|hfx
+      exact Or.inl ⟨x, hx, hfx⟩ 
+      exact Or.inr ⟨x, hx, hfx⟩ 
+    · rintro (⟨x, hx, hfx⟩|⟨x, hx, hfx⟩)
+      exact ⟨x, hx, mem_union _ _ _ |>.mpr (Or.inl hfx)⟩ 
+      exact ⟨x, hx, mem_union _ _ _ |>.mpr (Or.inr hfx)⟩ 
 
 theorem SetTheory.Set.preimage_of_diff {X Y:Set} (f:X → Y) (A B: Set) :
-    preimage f (A \ B) = (preimage f A) \ (preimage f B)  := by sorry
+  preimage f (A \ B) = (preimage f A) \ (preimage f B)  := by
+    ext x
+    simp_rw [mem_sdiff, mem_preimage']
+    push_neg
+    constructor
+    · rintro ⟨x, hx, h⟩ 
+      rw [mem_sdiff] at h
+      refine ⟨⟨x, hx, h.left⟩, fun x' hx' => ?_⟩ 
+      obtain rfl : x = x' := coe_inj _ _ _ |>.mp (hx ▸ hx'.symm)
+      exact h.right
+    · rintro ⟨⟨x, hx, hfx⟩, hnB⟩ 
+      exact ⟨x, hx, mem_sdiff _ _ _ |>.mpr ⟨hfx, hnB _ hx⟩⟩ 
 
 /-- Exercise 3.4.5 -/
 theorem SetTheory.Set.image_preimage_of_surj {X Y:Set} (f:X → Y) :
-    (∀ S, S ⊆ Y → image f (preimage f S) = S) ↔ Function.Surjective f := by sorry
+  (∀ S, S ⊆ Y → image f (preimage f S) = S) ↔ Function.Surjective f := by
+    constructor
+    · intro h y
+      replace h := h ({y.val}: Set) (fun _ h => (mem_singleton _ _ |>.mp h) ▸ y.prop)
+      replace h := Set.ext_iff.mp h
+      replace h := h y.val |>.mpr (mem_singleton _ _ |>.mpr rfl)
+      obtain ⟨x, _, hx⟩ := mem_image _ _ _ |>.mp h
+      exact ⟨x, coe_inj _ _ _ |>.mp hx⟩ 
+    · intro h S hS
+      ext y
+      rw [mem_image]
+      constructor
+      · intro ⟨x, hx, hf⟩ 
+        rw [mem_preimage] at hx
+        exact hf ▸ hx
+      · intro hy
+        obtain ⟨x, hx⟩ := h ⟨y, hS _ hy⟩ 
+        replace hx : ↑(f x) = y := by rw [hx]
+        refine ⟨x, ?_, hx⟩ 
+        rw [mem_preimage]
+        exact hx ▸ hy
 
 /-- Exercise 3.4.5 -/
 theorem SetTheory.Set.preimage_image_of_inj {X Y:Set} (f:X → Y) :
-    (∀ S, S ⊆ X → preimage f (image f S) = S) ↔ Function.Injective f := by sorry
+  (∀ S, S ⊆ X → preimage f (image f S) = S) ↔ Function.Injective f := by
+    unfold Function.Injective
+    constructor
+    · intro h x1 x2 hf
+      have h := h ({x1.val}: Set) (fun _ h => (mem_singleton _ _ |>.mp h) ▸ x1.prop)
+      rw [image_singleton', hf, Set.ext_iff] at h
+      replace h := h x2 |>.mp (by rw [mem_preimage, mem_singleton])
+      replace h := mem_singleton _ _ |>.mp h
+      exact (coe_inj _ _ _).mp h.symm
+    intro hf S hS
+    ext x
+    constructor
+    · intro hx
+      obtain ⟨x, rfl, h⟩ := mem_preimage' _ _ _ |>.mp hx
+      have ⟨x', hS, h⟩ := mem_image _ _ _ |>.mp h
+      have : x = x' := hf <| (coe_inj _ _ _).mp h.symm
+      exact this ▸ hS
+    · intro hx
+      rw [mem_preimage']
+      use ⟨x, hS _ hx⟩, rfl
+      rw [mem_image]
+      use ⟨x, hS _ hx⟩
 
 /-- Helper lemma for Exercise 3.4.7. -/
 @[simp]
@@ -331,40 +647,106 @@ lemma SetTheory.Set.mem_union_powerset_replace_iff {S : Set} {P : S.powerset →
 /-- Exercise 3.4.7 -/
 theorem SetTheory.Set.partial_functions {X Y:Set} :
     ∃ Z:Set, ∀ F:Object, F ∈ Z ↔ ∃ X' Y':Set, X' ⊆ X ∧ Y' ⊆ Y ∧ ∃ f: X' → Y', F = f := by
-  sorry
+    use union (Y.powerset.replace (P := fun Y'' outer =>
+        outer = union (X.powerset.replace (P := fun X'' inner =>
+          ∃ (X' Y': Set), Y''.val = ↑Y' ∧ X''.val = ↑X' ∧ inner = (Y' ^ X' :Set)
+        ) (by aesop))
+      ) (by aesop))
+    intro F
+    rw [mem_union_powerset_replace_iff]
+    constructor
+    · rintro ⟨Y'', outer, hY'', h_outer⟩ 
+      rw [Function.Embedding.injective set_to_object hY'', mem_union_powerset_replace_iff] at h_outer
+      obtain ⟨X'', inner, ⟨X', Y', hY', hX', h_inner⟩, hF⟩ := h_outer
+      refine ⟨X', Y', by aesop, by aesop, ?_⟩
+      rw [Function.Embedding.injective set_to_object h_inner, powerset_axiom] at hF
+      obtain ⟨f, hf⟩ := hF
+      use f, hf.symm
+    rintro ⟨X', Y', hX', hY', ⟨f, rfl⟩⟩ 
+    use ⟨Y', mem_powerset'.mpr hY'⟩
+    simp [mem_union_powerset_replace_iff]
+    grind only
 
 /--
   Exercise 3.4.8.  The point of this exercise is to prove it without using the
   pairwise union operation `∪`.
 -/
 theorem SetTheory.Set.union_pair_exists (X Y:Set) : ∃ Z:Set, ∀ x, x ∈ Z ↔ (x ∈ X ∨ x ∈ Y) := by
-  sorry
+  use union {↑X, ↑Y}
+  intro x
+  rw [union_axiom]
+  constructor
+  · rintro ⟨S, hx, hS⟩ 
+    obtain hS|hS := mem_pair _ _ _ |>.mp hS
+    exact (coe_eq_iff _ _).mp hS ▸ (Or.inl hx)
+    exact (coe_eq_iff _ _).mp hS ▸ (Or.inr hx)
+  · rintro (hx|hx)
+    exact ⟨X, hx, mem_pair _ _ _ |>.mpr (Or.inl rfl)⟩ 
+    exact ⟨Y, hx, mem_pair _ _ _ |>.mpr (Or.inr rfl)⟩ 
 
 /-- Exercise 3.4.9 -/
 theorem SetTheory.Set.iInter'_insensitive {I:Set} (β β':I) (A: I → Set) :
-    iInter' I β A = iInter' I β' A := by sorry
+  iInter' I β A = iInter' I β' A := by
+    ext x
+    unfold iInter'
+    rw [specification_axiom'', specification_axiom'']
+    constructor
+    · exact fun ⟨hx, h⟩ => ⟨h β', h⟩ 
+    · exact fun ⟨hx, h⟩ => ⟨h β, h⟩ 
+
 
 /-- Exercise 3.4.10 -/
 theorem SetTheory.Set.union_iUnion {I J:Set} (A: (I ∪ J:Set) → Set) :
-    iUnion I (fun α ↦ A ⟨ α.val, by simp [α.property]⟩)
-    ∪ iUnion J (fun α ↦ A ⟨ α.val, by simp [α.property]⟩)
-    = iUnion (I ∪ J) A := by sorry
+  iUnion I (fun α ↦ A ⟨ α.val, by simp [α.property]⟩)
+  ∪ iUnion J (fun α ↦ A ⟨ α.val, by simp [α.property]⟩)
+  = iUnion (I ∪ J) A := by
+    ext x
+    simp_rw [mem_union, mem_iUnion]
+    constructor
+    · rintro (⟨a, ha⟩|⟨a, ha⟩)
+      use ⟨ a.val, by simp [a.property]⟩
+      use ⟨ a.val, by simp [a.property]⟩
+    · rintro ⟨⟨a, ha⟩, h⟩
+      obtain ha|ha := mem_union _ _ _ |>.mp ha
+      exact Or.inl ⟨⟨a, ha⟩, h⟩ 
+      exact Or.inr ⟨⟨a, ha⟩, h⟩ 
 
 /-- Exercise 3.4.10 -/
-theorem SetTheory.Set.union_of_nonempty {I J:Set} (hI: I ≠ ∅) (hJ: J ≠ ∅) : I ∪ J ≠ ∅ := by sorry
+theorem SetTheory.Set.union_of_nonempty {I J:Set} (hI: I ≠ ∅) : I ∪ J ≠ ∅ := by
+  apply not_eq_iff.mpr
+  obtain ⟨x, hx⟩ := nonempty_def hI
+  refine ⟨x, ⟨fun _ => not_mem_empty _, fun _ => ?_⟩⟩
+  exact mem_union _ _ _ |>.mpr (Or.inl hx)
+
+theorem SetTheory.Set.union_of_nonempty' {I J:Set} (hJ: J ≠ ∅) : I ∪ J ≠ ∅ :=
+  union_comm _ _ ▸ union_of_nonempty hJ
+  
 
 /-- Exercise 3.4.10 -/
 theorem SetTheory.Set.inter_iInter {I J:Set} (hI: I ≠ ∅) (hJ: J ≠ ∅) (A: (I ∪ J:Set) → Set) :
-    iInter I hI (fun α ↦ A ⟨ α.val, by simp [α.property]⟩)
-    ∩ iInter J hJ (fun α ↦ A ⟨ α.val, by simp [α.property]⟩)
-    = iInter (I ∪ J) (union_of_nonempty hI hJ) A := by sorry
+  iInter I hI (fun α ↦ A ⟨ α.val, by simp [α.property]⟩)
+  ∩ iInter J hJ (fun α ↦ A ⟨ α.val, by simp [α.property]⟩)
+  = iInter (I ∪ J) (union_of_nonempty hI) A := by
+    ext x
+    simp_rw [mem_inter, mem_iInter]
+    refine ⟨fun ⟨h_mem_I, h_mem_J⟩ x' => ?_, fun h => ⟨fun x' => ?_, fun x' => ?_⟩⟩ 
+    · obtain hx'|hx' := mem_union _ _ _ |>.mp x'.prop
+      exact h_mem_I ⟨x'.val, hx'⟩ 
+      exact h_mem_J ⟨x'.val, hx'⟩ 
+    exact h ⟨x'.val, mem_union _ _ _ |>.mpr (Or.inl x'.prop)⟩ 
+    exact h ⟨x'.val, mem_union _ _ _ |>.mpr (Or.inr x'.prop)⟩ 
 
 /-- Exercise 3.4.11 -/
 theorem SetTheory.Set.compl_iUnion {X I: Set} (hI: I ≠ ∅) (A: I → Set) :
-    X \ iUnion I A = iInter I hI (fun α ↦ X \ A α) := by sorry
+  X \ iUnion I A = iInter I hI (fun α ↦ X \ A α) := by
+    ext x
+    have : Nonempty I.toSubtype := nonempty_subtype.mpr (nonempty_def hI)
+    simp_rw [mem_iInter, mem_sdiff, mem_iUnion, not_exists, forall_and_left]
 
 /-- Exercise 3.4.11 -/
 theorem SetTheory.Set.compl_iInter {X I: Set} (hI: I ≠ ∅) (A: I → Set) :
-    X \ iInter I hI A = iUnion I (fun α ↦ X \ A α) := by sorry
+  X \ iInter I hI A = iUnion I (fun α ↦ X \ A α) := by
+    ext x
+    simp_rw [mem_iUnion, mem_sdiff, mem_iInter, not_forall, exists_and_left]
 
 end Chapter3
