README.md
@@ -8,6 +8,7 @@ Heya, I have been going through the exercises and trying to fill in all the
   - Section 3.1
   - Section 3.2
   - Section 3.3
+  - Section 3.4
 
 
 # Lean formalization of _Analysis I_
